src/coq/optimisations/Kildall/congruence_proof_kildall.v
@@ -1,11 +1,12 @@
 Require Import ZArith List String Omega.
 Require Import  Vellvm.Ollvm_ast Vellvm.Classes Vellvm.Util Vellvm.CFGProp Vellvm.CFG.
-Require Import Vellvm.optimisations.transform.
 Require Import Vellvm.optimisations.paco_util.
 Require Import Vellvm.optimisations.step_trace.
 Require Import Vellvm.optimisations.Kildall.congruence_definition_kildall.
-Require Import Vellvm.optimisations.Kildall.static_eval_valueanalysis.
-Require Import Vellvm.optimisations.Kildall.static_eval_valuedomain.
+Require Import Vellvm.optimisations.Kildall.valueanalysis.
+Require Import Vellvm.optimisations.Kildall.valuedomain.
+Require Import Vellvm.optimisations.Kildall.static_eval.
+
 Require Import Vellvm.optimisations.maps.
 
 Print sound_state.
@@ -74,14 +75,11 @@ Ltac destr_eq t := destruct t eqn:?; simpl; eauto.
 Ltac destr t := destruct t; simpl; eauto.
 Ltac appl t y := generalize y; intro; apply t in y.
 
-
-
-
-
-
+Print Expr. Print typ. Print Ollvm_ast.typ.  Print instr.
+   
                                                                                                                                                                            
 Lemma congruence_correct1 : forall o m st mem (correct_instr: correct_instr1 o m) (wf_program: wf_program m) (sstate: sound_state m st), trace_equiv (memD mem (sem m st)) (memD mem (sem (modul_opt o m) st)).
-Proof.
+Proof. 
   pcofix CIH. intros. pfold.
   assert (memD mem (sem m st) = unroll(memD mem (sem m st))). destruct (memD mem (sem m st)); eauto. rewrite H. clear H.
   assert ( (memD mem (sem (modul_opt o m) st)) = unroll  (memD mem (sem (modul_opt o m) st))).
@@ -121,115 +119,24 @@ unfold exec_code1 in wf_program. simpl in *.
 rewrite  find_function_entry_unaffected_V1.
 inv sstate.
 unfold individual_step in *; simpl in *. destruct pt; simpl in *.
-destruct ( o {| fn := fn; bk := bk; pt := IId id |} m (IId id, i)), i; simpl in *; eauto; unfold  lift_err_d in *; try (repeat break_goal); try inv wf_program. 
+destruct ( o {| fn := fn; bk := bk; pt := IId id |} m (IId id, i)), i; simpl in *; eauto; unfold  lift_err_d in *; try (repeat break_goal); try inv wf_program.
+
+
+
+
+
+
   +assert (fetch m (mk_pc fn bk (IId id)) = Some (CFG.Step (INSTR_Op op0))). unfold fetch. simpl in *. rewrite Heqo0. rewrite Heqo1. rewrite Heqo2. eauto.
 
   +assert (incr_pc  m (mk_pc fn bk (IId id)) = Some (mk_pc fn bk i0)). unfold incr_pc; simpl. rewrite Heqo0. rewrite Heqo1. rewrite Heqo2. eauto.
 
 
    
-   constructor. right. eapply CIH; intros; eauto. destr_eq op0. simpl. destr_eq e0; eapply sound_succ_state; try apply AN; try rewrite H; simpl; unfold transfer'; try rewrite H; simpl; unfold get_successors; try rewrite H; try rewrite H0; simpl; eauto; try apply ematch_update; eauto; try constructor.
-assert (eval_op e None (SV (VALUE_Integer x)) = inr (DV (VALUE_Integer x))). simpl in *. eauto. rewrite Heqe0 in H1. inversion H1. eauto.
+   constructor. right. eapply CIH; intros; eauto; destr_eq op; destr_eq op0.
+subst. eapply sound_succ_state. eapply AN. eapply H. unfold get_successors; simpl in *; rewrite H; rewrite H0; simpl in *; left; eauto. unfold transfer'; rewrite H.  eauto. 
+apply ematch_update; eauto. 
 
-
-   
-
-
-
-
-
-
-
-  +eapply stack_false_l in H6. inversion H6.
-  +apply false_mem in H; inversion H.
-  +constructor; right; eapply CIH; intros; eauto. eapply sound_succ_state. eapply AN; auto.
-   unfold fetch; simpl in *; rewrite Heqo0; rewrite Heqo1; rewrite Heqo2; eauto. eauto. unfold transfer'; simpl in *; rewrite Heqo0; rewrite Heqo1; rewrite Heqo2; eauto. eapply ematch_update; eauto; constructor; eauto. eauto.
-  +SearchAbout stack. apply stack_false_r in H6. inversion H6.
-  +constructor. right. eapply CIH; intros; eauto. eapply sound_succ_state. eapply AN; eauto.
-   unfold fetch; simpl in *; rewrite Heqo0; rewrite Heqo1; rewrite Heqo2; eauto. unfold get_successors; simpl in *; rewrite Heqo0; rewrite Heqo1; rewrite Heqo2. unfold find_function_entry; simpl in *; rewrite Heqo3; rewrite Heqo4; simpl in *. eauto. unfold transfer'; simpl in *; rewrite Heqo0; rewrite Heqo1; rewrite Heqo2; eauto. constructor. econstructor; eauto. simpl in *; rewrite Heqo0; rewrite Heqo1; rewrite Heqo2; eauto.
-  +eapply stack_false_r in H7; inversion H7.
-  +eapply stack_false_r in H6; inversion H6.
-  +symmetry in H; eapply false_mem in H; inversion H.
-  +eapply stack_false_l in H7; inversion H7.
-  +constructor; right; eapply CIH; intros; eauto. eapply sound_succ_state. eapply AN.
-   unfold fetch; simpl in *; rewrite Heqo0; rewrite Heqo1; rewrite Heqo2; eauto. eauto.  
-   unfold transfer'; simpl in *; rewrite Heqo0; rewrite Heqo1; rewrite Heqo2; eauto.  eapply ematch_update; eauto; constructor; eauto. eauto.
-  +symmetry in H; eapply false_mem in H; inversion H.
-  +constructor; right; eapply CIH; intros; eauto. destruct op.
-
-
-
-
-  +assert (fetch m (mk_pc fn bk (IId id)) = Some (CFG.Step (INSTR_Op (SV e0)))). unfold fetch. simpl in *. rewrite Heqo0. rewrite Heqo1. rewrite Heqo2. eauto.
-
-  +assert (incr_pc  m (mk_pc fn bk (IId id)) = Some (mk_pc fn bk i0)). unfold incr_pc; simpl. rewrite Heqo0. rewrite Heqo1. rewrite Heqo2. eauto.
-
- destr_eq e0; eapply sound_succ_state; try apply AN; try rewrite H; simpl; unfold transfer'; try rewrite H; simpl; unfold get_successors; try rewrite H; try rewrite H0; simpl; eauto; try apply ematch_update; eauto; try constructor.
-assert (eval_op e None (SV (VALUE_Integer x)) = inr (DV (VALUE_Integer x))). simpl in *. eauto. rewrite Heqe0 in H1. inversion H1. eauto.
-
-
-
-
-
-  +eapply stack_false_l in H6; inversion H6.
-  +eapply false_mem in H; inversion H.
-  +constructor; right; eapply CIH; intros; eauto. eapply sound_succ_state. eapply AN.
-   unfold fetch; simpl in *; rewrite Heqo0; rewrite Heqo1; rewrite Heqo2; eauto. eauto.
-   unfold transfer'; simpl in *; rewrite Heqo0; rewrite Heqo1; rewrite Heqo2; eauto.  eapply ematch_update; eauto. constructor. eauto.
-
-
-
-   destruct ( o {| fn := fn; bk := bk; pt := IVoid n |} m (IVoid n, i)), i; simpl in *; eauto; unfold lift_err_d in *; simpl in *; try (repeat break_goal); try inv wf_program.
-
-  +constructor; right; eapply CIH; intros; eauto. eapply sound_succ_state. eapply AN.
-   unfold fetch; simpl in *; rewrite Heqo0; rewrite Heqo1; rewrite Heqo2; eauto. unfold get_successors; simpl in *; rewrite Heqo0; rewrite Heqo1; rewrite Heqo2; unfold find_function_entry; simpl in *; rewrite Heqo3; rewrite Heqo4; simpl in *; eauto. unfold transfer'; simpl in *; rewrite Heqo0; rewrite Heqo1; rewrite Heqo2; eauto. eauto. econstructor; eauto. exists (TYPE_Void, ID_Global id0). exists args0. exists n. simpl in *; rewrite Heqo0; rewrite Heqo1; rewrite Heqo2; simpl in *; eauto.
-  +eapply stack_false_r in H7; inversion H7.
-  +eapply stack_false_l in H7; inversion H7.
-  +constructor; right; eapply CIH; intros; eauto. eapply sound_succ_state. eapply AN. 
-   unfold fetch; simpl in *; rewrite Heqo0; rewrite Heqo1; rewrite Heqo2; eauto. eauto.
-   unfold transfer'; simpl in *; rewrite Heqo0; rewrite Heqo1; rewrite Heqo2; eauto.  eauto. eauto. eauto.
-
-
-
-
-
- rewrite jump_unaffected_v1.
-   destruct t; simpl in *; eauto.
-  + 
-    destruct v. destruct (eval_op e (Some t) v) eqn:?; simpl in *; eauto. destruct s; simpl in *; eauto. destruct f; simpl in *; eauto.
-
-
-
-
-
-    inversion sstate; subst; eauto. simpl in *. inversion sstack; subst; eauto. simpl in *. destruct H1. destruct H. destruct H. destruct q. simpl in *. destr_eq ( find_function m fn0). destr_eq ( find_block (blks (df_instrs d0)) bk0). destr_eq ( block_to_cmd b0 (IId id)). destruct p. destruct o1. simpl in *. inversion H0; subst. inversion H. subst. clear H. clear H0. constructor. right. eapply CIH; intros; eauto. eapply sound_succ_state. eapply AN0. unfold fetch; simpl in *; rewrite Heqo3; rewrite Heqo4; rewrite Heqo5; eauto. dupl Heqo3. eapply block_implies_successor in Heqo3; eauto. unfold transfer'; simpl in *; rewrite Heqo3; rewrite Heqo4; rewrite Heqo5; eauto. eauto. eauto. inversion H0. inversion H0. inversion H0. inversion H0.
-
-
-
-  +destruct s; simpl in *; eauto. destruct f; simpl in *; eauto. constructor; right; eapply CIH; intros; eauto. inversion sstate; subst; simpl in *; eauto; clear sstate. inversion sstack; simpl in *; subst; clear sstack. destruct H1. destruct H. destruct H. destruct H. destruct H0. destruct H1. destruct p. simpl in *. destr_eq (find_function m fn0). destr_eq (find_block (blks (df_instrs d0)) bk0). destr_eq ( block_to_cmd b0 (IVoid x1)). destruct p. destr o1. inversion H1; inversion H2; subst; clear H1; clear H2. eapply sound_succ_state. eapply H. unfold fetch; simpl in *; rewrite Heqo3; rewrite Heqo4; rewrite Heqo5; simpl in *; eauto. eauto. unfold transfer'; simpl in *; rewrite Heqo3; rewrite Heqo4; rewrite Heqo5; eauto. eauto. eauto. inversion H2. inversion H2. inversion H2. inversion H2.
-
-  +destruct v. destr_eq (eval_op e (Some t) v). destr_eq v0. destr_eq (StepSemantics.Int1.eq x StepSemantics.Int1.one). unfold jump; simpl in *. unfold find_block_entry; simpl in *.
-   destr_eq (find_function m fn). destr_eq ( find_block (blks (df_instrs d0)) br1). simpl in *.
-unfold monad_fold_right. simpl in *. destr_eq ( (fix
-                monad_fold_right (A B : Type) (M : Type -> Type) (H : Functor M) 
-                                 (H0 : Monad) (f : A -> B -> M A) (l : seq B) 
-                                 (a : A) {struct l} : M A :=
-                  match l with
-                  | [::] => mret a
-                  | x0 :: xs => monad_fold_right A B M H H0 f xs a ≫= (fun y : A => f y x0)
-                  end)). constructor. right. eapply CIH; intros; eauto. simpl in *. unfold blk_entry_pc. simpl in *. clear Heqp. inversion sstate; subst; simpl in *; eauto. inversion Heqo0. subst. unfold blk_entry_id. simpl in *. eapply sound_succ_state. eapply AN. unfold fetch; simpl in *. rewrite Heqo3. rewrite Heqo1. rewrite Heqo2. eauto. unfold get_successors; simpl in *; rewrite Heqo3; rewrite Heqo1; rewrite Heqo2; unfold next_term. unfold block_entry_pc. simpl in *. unfold find_block_entry; simpl in *. rewrite Heqo3. rewrite Heqo4. unfold block_to_entry; simpl in *. destr_eq (find_block (blks (df_instrs d)) br2). unfold transfer'; simpl in *; rewrite Heqo3; rewrite Heqo1; rewrite Heqo2. eauto. eauto. eauto.
-
-
-
-  +unfold jump; simpl in *; eauto. unfold find_block_entry; simpl in *.
-rewrite Heqo0. destr_eq (find_block (blks (df_instrs d)) br2). unfold monad_fold_right. destr_eq ( (fix
-                monad_fold_right (A B : Type) (M : Type -> Type) (H : Functor M) 
-                                 (H0 : Monad) (f : A -> B -> M A) (l : seq B) 
-                                 (a : A) {struct l} : M A :=
-                  match l with
-                  | [::] => mret a
-                  | x0 :: xs => monad_fold_right A B M H H0 f xs a ≫= (fun y : A => f y x0)
-                  end)). constructor; right; eapply CIH; intros; eauto.  inversion sstate; subst; simpl in *. eapply sound_succ_state. eapply AN. unfold fetch; simpl in *. rewrite Heqo0. rewrite Heqo1. rewrite Heqo2. eauto. unfold blk_entry_pc. unfold blk_entry_id. simpl in *. unfold blk_term_id. simpl in *. unfold get_successors; simpl in *; rewrite Heqo0; rewrite Heqo1; rewrite Heqo2; unfold next_term. unfold block_entry_pc. unfold find_block_entry; simpl in *. rewrite Heqo0. rewrite Heqo3. destr_eq ( find_block (blks (df_instrs d)) br1). unfold transfer'; simpl in *; rewrite Heqo0; rewrite Heqo1; rewrite Heqo2. eauto. eauto. eauto.
+destruct e1; simpl in *; eauto; try constructor; try inversion Heqe0; eauto; unfold eval_expr in *; unfold eval_aenv_expr; simpl in *; try destruct t; try destruct sz; try constructor; try destruct p; try constructor; try destruct p; try constructor. try destruct p; try constructor. try destruct p; try constructor. try destruct p; try constructor. try destruct p; try constructor. destruct p; try constructor. destruct v1; try constructor. destruct e1; try constructor. destruct v2; try constructor. destruct e1; try constructor.  simpl in *. inversion Heqe0. simpl. eauto. destruct v1; try constructor. destruct e1; try constructor. destruct v2; try constructor. destruct e1; try constructor; simpl in *; try inversion H2; try constructor. destruct v1; try constructor. destruct e1; try constructor. destruct v2; try constructor. destruct e1; try constructor; simpl in *. inversion H2; eauto. destruct p; try constructor.  destruct p; try constructor. destruct p; try constructor. destruct p; try constructor. destruct p; try constructor. destruct v1; try constructor. destruct e1; try constructor. destruct v2; try constructor. destruct e1; try constructor; simpl in *. inversion H2; eauto. destruct v1; try constructor. destruct e1; try constructor. destruct v2; try constructor. destruct e1; try constructor; simpl in *. inversion H2; eauto. destruct v1, v2; try constructor. destruct e1, e2; try constructor; simpl in *. inversion H2; eauto. eauto.
 
 
 
@@ -242,18 +149,150 @@ rewrite Heqo0. destr_eq (find_block (blks (df_instrs d)) br2). unfold monad_fold
 
 
 
-  +unfold jump; simpl in *; eauto. unfold find_block_entry; simpl in *.
-rewrite Heqo0. destr_eq (find_block (blks (df_instrs d)) br). unfold monad_fold_right. destr_eq ( (fix
-                monad_fold_right (A B : Type) (M : Type -> Type) (H : Functor M) 
-                                 (H0 : Monad) (f : A -> B -> M A) (l : seq B) 
-                                 (a : A) {struct l} : M A :=
-                  match l with
-                  | [::] => mret a
-                  | x0 :: xs => monad_fold_right A B M H H0 f xs a ≫= (fun y : A => f y x0)
-                  end)). constructor; right; eapply CIH; intros; eauto.  inversion sstate; subst; simpl in *. eapply sound_succ_state. eapply AN. unfold fetch; simpl in *. rewrite Heqo0. rewrite Heqo1. rewrite Heqo2. eauto. unfold blk_entry_pc. unfold blk_entry_id. simpl in *. unfold blk_term_id. simpl in *. unfold get_successors; simpl in *; rewrite Heqo0; rewrite Heqo1; rewrite Heqo2; unfold next_term. unfold block_entry_pc. unfold find_block_entry; simpl in *. rewrite Heqo0. rewrite Heqo3. unfold block_to_entry; simpl in *; eauto. unfold transfer'; simpl in *; rewrite Heqo0; rewrite Heqo1; rewrite Heqo2; eauto. eauto. eauto. Qed.
 
-SearchAbout ematch.
-Print AE.get.
-Print aval. Print lookup_env.
-Lemma ematch_get : forall e a id val, ematch e a -> AE.get id a = avalue val -> lookup_env e id = Some val.
-  Proof. intros. unfold ematch in *. simpl in *. specialize (H id). rewrite H0 in H. simpl in *. inversion H; subst. unfold lookup_env_aenv in *. simpl in *. destr_eq (lookup_env e id). inversion H1. subst. eauto. inversion H1. Qed.
+
+eapply stack_false_l in H6; inversion H6.
+eapply mem_false_l in H; inversion H.
+
+
+
+
+
+
+constructor. right. eapply CIH; intros; eauto. eapply sound_succ_state; try eapply AN.
+unfold fetch; simpl in *; rewrite Heqo0; rewrite Heqo1; try rewrite Heqo2; eauto.
+unfold get_successors; simpl in *; rewrite Heqo0; rewrite Heqo1; rewrite Heqo2; simpl in *; eauto.
+unfold transfer'; simpl in *; rewrite Heqo0; rewrite Heqo1; rewrite Heqo2; eauto.
+eapply ematch_update; eauto; try constructor. eauto.
+
+
+
+
+eapply stack_false_r in H6; inversion H6.
+constructor. right. eapply CIH; intros; eauto. eapply sound_succ_state. eapply AN. unfold fetch. rewrite Heqo0; simpl in *; rewrite Heqo1; rewrite Heqo2; eauto. unfold get_successors; simpl in *; rewrite Heqo0; rewrite Heqo1; rewrite Heqo2; unfold find_function_entry; simpl in *; rewrite Heqo5; simpl in ; rewrite Heqo6; simpl in *; inversion H4; inversion H3; subst; eauto. unfold transfer'; simpl in *; rewrite Heqo0; try rewrite Heqo1; try rewrite Heqo2; eauto. eauto. econstructor; simpl in *; eauto. rewrite Heqo0; rewrite Heqo1; rewrite Heqo2; eauto.
+
+
+eapply stack_false_r in H7; inversion H7.
+eapply stack_false_r in H6; inversion H6.
+symmetry in H; eapply mem_false_l in H; inversion H.
+eapply stack_false_l in H7; inversion H7.
+
+
+constructor. right. eapply CIH; intros; eauto. eapply sound_succ_state. eapply AN. unfold fetch; simpl; rewrite Heqo0; rewrite Heqo1; rewrite Heqo2; eauto. unfold get_successors; simpl in *; rewrite Heqo0; rewrite Heqo1; rewrite Heqo2; simpl in *; eauto. unfold transfer'; unfold fetch; simpl; rewrite Heqo0; rewrite Heqo1; rewrite Heqo2; eauto. eapply ematch_add; eauto. eauto.
+
+
+symmetry in H; eapply mem_false_l in H; inversion H.
+
+destr_eq op.
+
+constructor. right. eapply CIH; intros; eauto. eapply sound_succ_state. eapply AN. unfold fetch; simpl; rewrite Heqo0; rewrite Heqo1; rewrite Heqo2; eauto. unfold get_successors; simpl in *; rewrite Heqo0; rewrite Heqo1; rewrite Heqo2; simpl in *; eauto. unfold transfer'; unfold fetch; simpl in *; rewrite Heqo0; rewrite Heqo1; rewrite Heqo2; eauto. unfold add_env. simpl in *. unfold eval_aenv_expr; simpl in *; destr_eq e0; simpl in *; try destr_eq t1; try inv Heqe0;
+
+                                                                                                                                                                                                                                                                                                                                                                                             try destr_eq sz; try destr_eq p; try destr_eq p0; try destr_eq p1; try destr_eq p2; try destr_eq p3; try destr_eq p4; try destr_eq p5; try destr_eq v1; try destr_eq e0; try destr_eq v2; try destr_eq e1; try inv H0; try eapply ematch_update; eauto; constructor; eauto. eauto.
+
+
+
+eapply stack_false_l in H6; inversion H6.
+eapply mem_false_l in H; inversion H; eauto.
+
+
+constructor; right; eapply CIH; intros; eauto.
+
+
+eapply sound_succ_state. eapply AN. unfold fetch; simpl in *; rewrite Heqo0; rewrite Heqo1; rewrite Heqo2; simpl in *; eauto. unfold get_successors; simpl in *; rewrite Heqo0; rewrite Heqo1; rewrite Heqo2; simpl in *; eauto.
+
+
+unfold transfer'; simpl in *; eauto; rewrite Heqo0; rewrite Heqo1; rewrite Heqo2; eauto. eapply ematch_add; eauto. eauto.
+
+
+
+destr_eq ( o {| fn := fn; bk := bk; pt := IVoid n |} m (IVoid n, i)); destr_eq i; simpl in *; eauto; unfold  lift_err_d in *; try (repeat break_goal); try inv wf_program; try eapply stack_false_r in H7; try inv H7; try eapply stack_false_l in H7; try inv H7; try constructor; try right; try eapply CIH; intros; eauto.
+
+
+
+
+
+eapply sound_succ_state; try eapply AN; unfold fetch; unfold transfer'; unfold get_successors; simpl; try rewrite Heqo0; try rewrite Heqo1; try rewrite Heqo2; auto; unfold find_function_entry; simpl in *; try rewrite Heqo5; try rewrite Heqo6; simpl. rewrite H4. right. left. rewrite H3. eauto.
+
+
+
+
+
+econstructor; eauto. simpl in *. rewrite Heqo0. rewrite Heqo1. exists (TYPE_Void, ID_Global id0), args0, n. rewrite Heqo2. eauto.
+
+
+
+
+
+
+eapply stack_false_l in H0. inversion H0.
+
+
+
+
+
+
+
+
+
+eapply sound_succ_state; try eapply AN. unfold fetch; simpl in *. rewrite Heqo0. rewrite Heqo1. rewrite Heqo2. eauto. unfold get_successors; simpl in *. rewrite Heqo0; rewrite Heqo1; rewrite Heqo2; simpl; eauto. unfold transfer'. simpl in *. rewrite Heqo0; rewrite Heqo1; rewrite Heqo2. eauto.
+eauto. eauto.
+
+
+
+
+
+
+
+
+
+
+
+
+
+
+
+
+
+
+
+
+auto.
+
+
+
+
+rewrite jump_unaffected_v1.
+
+unfold jump. destruct t; unfold  lift_err_d in *; try (repeat break_goal); subst; try inv Heqt; constructor; right; eapply CIH; intros; eauto; inv sstate. simpl in EM; simpl in AN; simpl in sstack.
+
+inv sstack. simpl in *. destruct q. simpl in *. destruct H1. destruct H. destruct H. destr_eq (find_function m fn0). destr_eq ( find_block (blks (df_instrs d0)) bk0). destr_eq (block_to_cmd b0 (IId id)). destr_eq p. simpl in *. destr_eq c. inv H. destr_eq o1. inv  H0. eapply sound_succ_state. eapply AN0. unfold fetch; simpl. rewrite Heqo3. rewrite Heqo4. rewrite Heqo5. eauto. unfold get_successors; simpl in *; rewrite Heqo3; rewrite Heqo4; rewrite Heqo5. simpl in *. destruct x. simpl in *. destruct i. simpl in *. unfold find_function_entry; simpl. destr_eq (find_function m id0).
+destr_eq ( find_block (blks (df_instrs d1)) (init (df_instrs d1))). simpl in *. eauto. unfold transfer'; simpl in *. rewrite Heqo3. rewrite Heqo4. rewrite Heqo5. eauto. simpl in *. eauto. eauto.
+inversion H0. inversion H. inversion H. inversion H. inversion H.
+
+
+
+simpl in *. inv sstack. simpl in *. destr H1. destr H. destr H. destr H. destr H0. destr H1. destr p. simpl in *. destr_eq (find_function m fn0). destr_eq ( find_block (blks (df_instrs d0)) bk0). destr_eq (block_to_cmd b0 (IVoid x1)). destr p. destr o1. inv H1. inv H2. eapply sound_succ_state.
+eapply H. unfold fetch; simpl. rewrite Heqo3. rewrite Heqo4. rewrite Heqo5. eauto. unfold get_successors; simpl in *. rewrite Heqo3. rewrite Heqo4. rewrite Heqo5. unfold find_function_entry. destr x. destr i. destr_eq (find_function m id). destr_eq ( find_block (blks (df_instrs d1)) (init (df_instrs d1))). unfold transfer'; simpl. rewrite Heqo3. rewrite Heqo4. rewrite Heqo5. simpl in *. eauto. eauto. eauto. inversion H1. inversion H2. inversion H1. inversion H1. inversion H1.
+
+
+
+
+
+simpl in *. eapply sound_succ_state. eapply AN.  unfold get_successors. simpl in *. rewrite Heqo0. rewrite Heqo1. rewrite Heqo2. eauto. unfold get_successors. simpl in *. unfold next_term. unfold block_entry_pc. simpl in *.  rewrite Heqo0. rewrite Heqo1. rewrite Heqo2. rewrite Heqo3. simpl. eauto. unfold transfer'. simpl in *. rewrite Heqo0. rewrite Heqo1. rewrite Heqo2. eauto. eauto. eauto.
+
+
+
+
+simpl in *. eapply sound_succ_state. eapply AN.  unfold get_successors. simpl in *. rewrite Heqo0. rewrite Heqo1. rewrite Heqo2. eauto. unfold get_successors. simpl in *. unfold next_term. unfold block_entry_pc. simpl in *.  rewrite Heqo0. rewrite Heqo1. rewrite Heqo2. rewrite Heqo3.
+destr_eq ( find_block_entry m fn br1). destr b0.
+unfold transfer'. simpl in *. rewrite Heqo0. rewrite Heqo1. rewrite Heqo2. eauto. eauto. eauto.
+
+
+
+
+
+
+simpl in *.  eapply sound_succ_state. eapply AN.  unfold get_successors. simpl in *. rewrite Heqo0. rewrite Heqo1. rewrite Heqo2. eauto. unfold get_successors. simpl in *. unfold next_term. unfold block_entry_pc. simpl in *.  rewrite Heqo0. rewrite Heqo1. rewrite Heqo2. rewrite Heqo3. simpl in *; eauto.
+unfold transfer'. simpl in *. rewrite Heqo0. rewrite Heqo1. rewrite Heqo2. eauto. eauto. eauto.
+
+Qed.
