src/coq/optimisations/StaticAnalysis/const_prop.v
@@ -1,6 +1,5 @@
 Require Import ZArith List String Omega.
 Require Import Vellvm.Ollvm_ast Vellvm.Classes Vellvm.Util Vellvm.CFGProp Vellvm.CFG.
-Require Import Vellvm.optimisations.transform.
 Require Import Vellvm.optimisations.paco_util.
 Require Import Vellvm.optimisations.step_trace.
 Require Import Vellvm.optimisations.EqNat.
